\documentclass{article}
\usepackage{epsfig}
\pagestyle{empty}
\begin{document}
$ v^{th} $
\pagebreak

$ n^{th} $
\pagebreak

$ 8 \le n < 20 $
\pagebreak

$ j^{th} $
\pagebreak

$ i^{th} $
\pagebreak

$ 8 \le n < 27 $
\pagebreak

$ 6^{th} $
\pagebreak

$ 8 \le n < 16 $
\pagebreak

$ 8 \le n < 18 $
\pagebreak

$ 5^{th} $
\pagebreak

$ 6 \le n < 12 $
\pagebreak

$ 6 \le n < 15 $
\pagebreak

$ 6 \le n < 18 $
\pagebreak

$ 4 \le n < 10 $
\pagebreak

$ Ay=G_{\lambda} $
\pagebreak

$ Az = -G $
\pagebreak

$\mathbf{a}$
\pagebreak

$\mathbf{b}$
\pagebreak

\[ (\mathbf{a}\mathbf{b}^T)_{i,j} = \mathbf{a}_i \mathbf{b}_j . \]
\pagebreak

\[ (\mathbf{a}\mathbf{b}^H)_{i,j} = \mathbf{a}_i \mathbf{b}^*_j , \]
\pagebreak

$H$
\pagebreak

$*$
\pagebreak

$ |M|_1 = max_{all columns j} \sum_{all rows i} |M_ij| $
\pagebreak

$ |Mv|_1 \leq |M|_1 |v|_1 $
\pagebreak

$ |M|_\infty = max_{all rows i} \sum_{all columns j} |M_ij| $
\pagebreak

$ |Mv|_\infty \leq |M|_\infty |v|_\infty $
\pagebreak

$ A x = rhs $
\pagebreak

$ x $
\pagebreak

$ A $
\pagebreak

$ u_j $
\pagebreak

$ u_j^H A = lambda_j u_j^H $
\pagebreak

$ u_j^H $
\pagebreak

$ v_j $
\pagebreak

$ A v_j = lambda_j v_j $
\pagebreak

$ lambda_j $
\pagebreak

$(m \times n)$
\pagebreak

$(0,0)$
\pagebreak

$(ioff,joff)$
\pagebreak

$l_1$
\pagebreak

$l_2$
\pagebreak

$l_\infty$
\pagebreak

\[ F(u) + G(u) - M(u,\dot{u})\dot{u} = 0 \]
\pagebreak

$ F(u) = 0$
\pagebreak

$F(u)$
\pagebreak

$ G(u) $
\pagebreak

$ M(u,\dot{u})\dot{u} $
\pagebreak

\[ M(u,\ddot{u})\ddot{u} + C(u,\dot{u})\dot{u} + F(u) + G(u) = 0 \]
\pagebreak

$G(u)$
\pagebreak

$C(u,\dot{u})\dot{u}$
\pagebreak

$ -M(u,\ddot{u})\ddot{u}$
\pagebreak

${u}$
\pagebreak

$\dot{u}$
\pagebreak

$\ddot{u}$
\pagebreak

$ u_{n+1} $
\pagebreak

$ M(u,\ddot{u})\ddot{u} $
\pagebreak

$ C(u,\ddot{u})\ddot{u} $
\pagebreak

$ Ue[i] = Ug[dof_indices[i]] $
\pagebreak

$ 4 \le n < 6 $
\pagebreak

$ 4 \le n < 8 $
\pagebreak

$ 3 \le n < 6 $
\pagebreak

$ C^1 $
\pagebreak

$ \{ p_n \} $
\pagebreak

$ \|p - p_n\| < \mbox{\texttt{tolerance}} $
\pagebreak

$ x \le 1 $
\pagebreak

$ x \le 1 + \epsilon $
\pagebreak

$ 1/{r^2} $
\pagebreak

$ \xi \le 1 $
\pagebreak

$ \xi \le 1 + \epsilon $
\pagebreak

$ t_{\theta} $
\pagebreak

\[ M(u)\dot{u} = F(u)\]
\pagebreak

\[ M(u)\ddot{u} + C(u)\dot{u} + F(u) = 0 \]
\pagebreak

$\dot{u} = v$
\pagebreak

\begin{eqnarray} \dot{u} &=& v \\ M(u)\dot{v} + C(u)v + F(u) &=& 0\end{eqnarray}
\pagebreak

$u$
\pagebreak

$v$
\pagebreak

$ \dot{u} = v$
\pagebreak

$ M(u)\dot{v} + C(u)v + F(u) = 0 $
\pagebreak

$ \dot{u} - v = 0 $
\pagebreak

$ u $
\pagebreak

$ v $
\pagebreak

$ [ \texttt{n\_start, n\_stop} ]^{th} $
\pagebreak

$ [ \texttt{min\_freq, max\_freq} ] $
\pagebreak

$ f(\mathbf{x},t) = \mbox{\texttt{v}} $
\pagebreak

$ \phi(x) = \phi(\xi) $
\pagebreak

$ H(curl) $
\pagebreak

$ \phi = (dx/d\xi)^{-T} \hat{\phi} $
\pagebreak

$ (dx/d\xi)^{-T} $
\pagebreak

$ x, \xi $
\pagebreak

$ \nabla \times \phi = J^{-1} * \nabla \times \hat{\phi} $
\pagebreak

$ J = \det( dx/d\xi ) $
\pagebreak

$ \nabla \times \phi = J^{-1} dx/d\xi \nabla \times \hat{\phi} $
\pagebreak

$ \ge 1 $
\pagebreak

$ 1/r $
\pagebreak

$ (i,j) $
\pagebreak

$ \sqrt{-1} $
\pagebreak

$ \pi=3.14159... $
\pagebreak

$ zero=0. $
\pagebreak

$ nx \times ny \times nz $
\pagebreak

$ [0,1] $
\pagebreak

$\gamma$
\pagebreak

$\beta$
\pagebreak

$a_0$
\pagebreak

$\gamma=0.5$
\pagebreak

$ \beta $
\pagebreak

$ \gamma $
\pagebreak

$ \gamma = 1/2 $
\pagebreak

$ \beta \ge \frac{1}{4} \left( \gamma + \frac{1}{2}\right)^2 $
\pagebreak

$ R(X) $
\pagebreak

$ J(X) $
\pagebreak

$ X $
\pagebreak

$ XL $
\pagebreak

$ XU $
\pagebreak

$ \ell_1 $
\pagebreak

$ \ell_2 $
\pagebreak

$ \ell_{\infty} $
\pagebreak

$ \vec{u} \leftarrow \vec{u} + \vec{v} $
\pagebreak

$ \vec{u} \leftarrow \vec{u} - \vec{v} $
\pagebreak

$ \vec{u} \leftarrow a\vec{u} $
\pagebreak

$ \vec{u} \leftarrow \frac{1}{a}\vec{u} $
\pagebreak

$ u_i \leftarrow \frac{u_i}{v_i} \, \forall i$
\pagebreak

$ u_i \leftarrow \frac{1}{u_i} \, \forall i$
\pagebreak

$ u_i \leftarrow u_i + s $
\pagebreak

$ \vec{u} \leftarrow \vec{u} + a\vec{v} $
\pagebreak

$ \vec{u} \leftarrow \vec{u} + A \vec{v} $
\pagebreak

$ \vec{u} \leftarrow \vec{u} + A^T \vec{v} $
\pagebreak

$ u_i \leftarrow |u_i| $
\pagebreak

$ \vec{u} \cdot \vec{v} $
\pagebreak

$ u_i \leftarrow u_i v_i $
\pagebreak

$ U \leftarrow U + A^H v $
\pagebreak

$ Py=x $
\pagebreak

$ P^-1 x $
\pagebreak

$ \frac{1}{V} \sum \|w_i\|, $
\pagebreak

$ \mu $
\pagebreak

$\dot{u}_n$
\pagebreak

$\ddot{u}_n$
\pagebreak

$ \dot{u}_n $
\pagebreak

$ \ddot{u}_n $
\pagebreak

$ M \times N $
\pagebreak

$ ||A x - \lambda x|| / |\lambda x| $
\pagebreak

$ A \leftarrow A + a*X $
\pagebreak

$ |M|_1 = \max_{j} \sum_{i} |M_{ij}| $
\pagebreak

$ |M|_{\infty} = \max_{i} \sum_{j} |M_{ij}| $
\pagebreak

$ |Mv|_{\infty} \leq |M|_{\infty} |v|_{\infty} $
\pagebreak

$ (x, y, z) $
\pagebreak

$ (r, \theta, \phi) $
\pagebreak

$ 0 \le r < \infty $
\pagebreak

$ 0 \le \theta < \pi $
\pagebreak

$ 0 \le \phi < 2\pi $
\pagebreak

$ \phi $
\pagebreak

$ \theta $
\pagebreak

$ \sum_{ij} A_{ij} B_{ij} $
\pagebreak

$ i,this $
\pagebreak

\end{document}
